Cleaned up warnings, removed old Nat utils

LogicalRefinement/Utils.lean
@@ -1,293 +1,6 @@
-import Init.Data.Nat
-
-def Nat.le_lt_succ (p: n ≤ m): (n < succ m) := Nat.lt_succ_of_le p
-
-def Nat.le_or_lt (l r: Nat): l < r ∨ r ≤ l := by {
-  cases Nat.le_total l r with
-  | inl Hlr => 
-    cases (Nat.decEq l r).em with
-    | inl Heq => apply Or.inr; rw [Heq]; apply Nat.le_refl
-    | inr Hne => exact Or.inl (Nat.lt_of_le_of_ne Hlr Hne)
-  | inr Hrl => exact Or.inr Hrl
-}
-
-def Nat.eq_zero_is_le_zero: (m ≤ 0) = (m = 0) := 
-  propext (Iff.intro Nat.eq_zero_of_le_zero Nat.le_of_eq)
-
-def Nat.succ_le_is_le: (succ m ≤ succ n) = (m ≤ n) := 
-  propext (Iff.intro Nat.le_of_succ_le_succ Nat.succ_le_succ)
-
-@[simp]
-def Nat.max_zero_left: {m: Nat} -> Nat.max m 0 = m
-  | 0 => rfl
-  | Nat.succ n => by { 
-    unfold Nat.max
-    unfold max
-    unfold instMaxNat
-    unfold maxOfLe
-    simp
-  }
-
-@[simp]
-def Nat.max_zero_right: {m: Nat} -> Nat.max 0 m = m
-  | 0 => rfl
-  | Nat.succ n => by { 
-    unfold Nat.max
-    unfold max
-    unfold instMaxNat
-    unfold maxOfLe
-    simp
-  }
-
-@[simp]
-def Nat.max_bin_succ: Nat.max (Nat.succ l) (Nat.succ r) = Nat.succ (Nat.max l r) := by {
-  unfold Nat.max
-  unfold max
-  unfold instMaxNat
-  unfold maxOfLe
-  simp
-  cases (Nat.decLe l r).em with
-  | inl Ht => 
-    rw [if_pos Ht]
-    rw [if_pos (Nat.succ_le_succ Ht)]
-  | inr Ht => 
-    rw [if_neg Ht]
-    rw [if_neg (λAht => Ht (Nat.le_of_succ_le_succ Aht))]
-}
-
-@[simp]
-def Nat.max_idempotent {l: Nat}: Nat.max l l = l := by {
-  unfold Nat.max
-  unfold max
-  unfold instMaxNat
-  unfold maxOfLe
-  simp
-}
-
-def Nat.max_val_l {l r: Nat} (p: r ≤ l): Nat.max l r = l := by {
-  unfold Nat.max
-  unfold max
-  unfold instMaxNat
-  unfold maxOfLe
-  simp
-  cases (Nat.decLe l r).em with
-  | inl Ht =>
-    rw [if_pos Ht]
-    exact Nat.le_antisymm p Ht
-  | inr Hf =>
-    rw [if_neg Hf]
-}
-
-def Nat.max_val_r {l r: Nat} (p: l ≤ r): Nat.max l r = r := by {
-  unfold Nat.max
-  unfold max
-  unfold instMaxNat
-  unfold maxOfLe
-  simp
-  rw [if_pos]
-  exact p
-}
-
-def Nat.max_le_l {l r: Nat}: l ≤ Nat.max l r := by {
-  unfold Nat.max
-  unfold max
-  unfold instMaxNat
-  unfold maxOfLe
-  simp
-  cases (Nat.decLe l r).em with
-  | inl Ht =>
-    rw [if_pos Ht]
-    apply Ht
-  | inr Hf =>
-    rw [if_neg Hf]
-    apply Nat.le_refl
-}
- 
-def Nat.max_le_r {l r: Nat}: r ≤ Nat.max l r := by {
-  unfold Nat.max
-  unfold max
-  unfold instMaxNat
-  unfold maxOfLe
-  simp
-  cases (Nat.decLe l r).em with
-  | inl Ht =>
-    rw [if_pos Ht]
-    apply Nat.le_refl
-  | inr Hf =>
-    rw [if_neg Hf]
-    cases (Nat.le_total l r) with
-    | inl Hlr => exact absurd Hlr Hf
-    | inr Hrl => exact Hrl
-}
-
-def Nat.max_r_le_split: (Nat.max l r ≤ m) = (l ≤ m ∧ r ≤ m) := by {
-  apply propext;
-  apply Iff.intro;
-  case a.mp =>
-    intro Hm
-    exact ⟨Nat.le_trans max_le_l Hm, Nat.le_trans max_le_r Hm⟩
-  case a.mpr =>
-    intro ⟨Hl, Hr⟩
-    cases Nat.le_total l r with
-    | inl Hlr => 
-      rw [Nat.max_val_r Hlr]
-      apply Hr
-    | inr Hrl =>
-      rw [Nat.max_val_l Hrl]
-      apply Hl
-}
-
-def Nat.max_l_le_split: (m ≤ Nat.max l r) = (m ≤ l ∨ m ≤ r) := by {
-  apply propext;
-  apply Iff.intro;
-  case a.mp =>
-    intro Hm
-    let Hlr: r ≤ l ∨ l ≤ r := Nat.le_total r l;
-    cases Hlr with
-    | inl Hlr =>
-      apply Or.inl;
-      rw [<-(@Nat.max_val_l l r)]
-      exact Hm
-      exact Hlr
-    | inr Hlr => 
-      apply Or.inr;
-      rw [<-(@Nat.max_val_r l r)]
-      exact Hm
-      exact Hlr
-  case a.mpr =>
-    intro Hm
-    cases Hm with
-    | inl Hm => exact Nat.le_trans Hm max_le_l
-    | inr Hm => exact Nat.le_trans Hm max_le_r
-}
-
-def Nat.max_r_lt_split: (Nat.max l r < m) = (l < m ∧ r < m) := by {
-  apply propext;
-  apply Iff.intro;
-  case a.mp =>
-    intro Hm
-    apply And.intro
-    case left =>
-      exact Nat.lt_of_le_of_lt Nat.max_le_l Hm
-    case right => 
-      exact Nat.lt_of_le_of_lt Nat.max_le_r Hm
-  case a.mpr =>
-    intro ⟨Hl, Hr⟩
-    cases Nat.le_total l r with
-    | inl Hlr =>
-      rw [Nat.max_val_r Hlr]
-      exact Hr
-    | inr Hlr =>
-      rw [Nat.max_val_l Hlr]
-      exact Hl
-}
-
-def Nat.max_l_lt_split: (m < Nat.max l r) = (m < l ∨ m < r) := by {
-  apply propext;
-  apply Iff.intro;
-  case a.mp =>
-    intro Hm
-    cases Nat.le_total l r with
-    | inl Hlr =>
-      apply Or.inr
-      rw [<-Nat.max_val_r Hlr]
-      apply Hm
-    | inr Hlr =>
-      apply Or.inl
-      rw [<-Nat.max_val_l Hlr]
-      apply Hm
-  case a.mpr =>
-    intro Hm
-    cases Hm with
-    | inl Hl => exact Nat.le_trans Hl Nat.max_le_l
-    | inr Hr => exact Nat.le_trans Hr Nat.max_le_r
-}
-
-private def Nat.succ_right: n + Nat.succ l = Nat.succ (n + l) := rfl
-
-def Nat.succ_le_succ_is_le: (succ n ≤ succ m) = (n ≤ m) :=
-  propext (Iff.intro Nat.le_of_succ_le_succ Nat.succ_le_succ)
-
-def Nat.succ_lt_succ_is_lt: (succ n < succ m) = (n < m) :=
-  propext (Iff.intro Nat.le_of_succ_le_succ Nat.succ_le_succ)
-
-def Nat.zero_le_true: (0 ≤ n) = True :=
-  propext (Iff.intro (λ _ => True.intro) (λ _ => Nat.zero_le _))
-
-def Nat.le_sub_is_le_add: {l n m: Nat} -> (n - l ≤ m) = (n ≤ m + l) := by {
-  intros l;
-  induction l with
-  | zero => intros; rfl
-  | succ l I => intros n; cases n with
-    | zero => {
-      intros m;
-      rw [Nat.zero_sub];
-      rw [Nat.zero_le_true];
-      rw [Nat.zero_le_true]
-    }
-    | succ n => {
-      intros m;
-      rw [Nat.succ_sub_succ_eq_sub];
-      rw [Nat.succ_right];
-      rw [Nat.succ_le_succ_is_le];
-      apply I
-    }
-}
-
-def Nat.lt_is_succ_le: {n m: Nat} -> (n < m) = (Nat.succ n ≤ m) := rfl
-
-def Nat.le_antistep: succ n ≤ l -> n ≤ l := by {
-  intro H;
-  induction H with
-  | refl => apply Nat.le_step; apply Nat.le_refl
-  | @step m _ I => apply Nat.le_step; apply I
-}
-
-def Nat.lt_antistep: succ n < l -> n < l := Nat.le_antistep
-
-def Nat.lt_l_add_lt: {n m l: Nat} -> n + m < l -> n < l := by {
-  intros n m;
-  induction m with
-  --TODO: report unused variable bug here
-  | zero => intros _ H; exact H
-  | succ m I => 
-    intros l H;
-    apply I
-    apply Nat.lt_antistep
-    rw [<-Nat.add_succ]
-    apply H
-}
-
-def Nat.lt_r_add_lt: {n m l: Nat} -> n + m < l -> m < l := by {
-  intros n m l;
-  rw [Nat.add_comm]
-  apply Nat.lt_l_add_lt
-}
-
-def Nat.lt_sub_lt_add: {l n m: Nat} -> n + m < l -> n < l - m := by {
-  intros l;
-  induction l with
-  | zero => 
-    intros n m H; 
-    rw [Nat.zero_sub]
-    apply Nat.lt_l_add_lt H
-  | succ l Hl =>
-    intros n m H;
-    cases H with
-    | refl =>
-      let H': succ (n + m) = (succ n) + m := by {
-        rw [Nat.add_comm]
-        rw [<-Nat.add_succ]
-        rw [Nat.add_comm]
-      }
-      rw [H']
-      rw [Nat.add_sub_self_right]
-      apply Nat.le_refl
-    | step H =>
-      apply Nat.le_trans _ (Nat.sub_le_succ_sub _ _)
-      apply Hl
-      apply H
-}
+import Std.Data.Nat.Init.Lemmas
+import Mathlib.Init.Data.Nat.Lemmas
+import Mathlib.Init.Order.LinearOrder
 
 theorem function_splitting {f g: A -> B}: f = g /\ x = y -> f x = g y := by {
   intro ⟨Hf, Hxy⟩;
@@ -295,54 +8,8 @@ theorem function_splitting {f g: A -> B}: f = g /\ x = y -> f x = g y := by {
   rw [Hxy]
 }
 
-def Nat.succ_match_simp {F: Nat -> A}: (v: Nat) -> (
-  match v + 1 with
-  | 0 => e
-  | Nat.succ n => F n 
-) = F v := λ_ => rfl
-
-theorem Nat.succ_sub_gt: {n m: Nat} -> m ≤ n -> n + 1 - m = (n - m) + 1 := by {
-  intro n;
-  induction n with
-  | zero =>
-    intro m
-    rw [Nat.eq_zero_is_le_zero]
-    intro H
-    rw [H]
-  | succ n I =>
-    intro m H
-    rw [Nat.add_succ, Nat.add_zero]
-    cases m with
-    | zero => simp
-    | succ m =>
-      repeat rw [Nat.succ_sub_succ_eq_sub]
-      exact I (Nat.le_of_succ_le_succ H)
-}
-
-theorem Nat.add_sub_self_gt: {n m: Nat} -> m ≤ n -> n - m + m = n := by {
-  intro n m;
-  induction m with
-  | zero => intros; rfl
-  | succ m I =>
-    intro H
-    cases n with
-    | zero => cases H
-    | succ n =>
-      rw [Nat.succ_le_succ_is_le] at H
-      rw [succ_sub_succ_eq_sub]
-      rw [add_succ]
-      let R: succ (n - m + m) = n - m + 1 + m := by {
-        rw [Nat.add_assoc]
-        rw [@Nat.add_comm 1 m]
-        rfl
-      }
-      rw [R]
-      rw [<-Nat.succ_sub_gt H]
-      exact I (Nat.le_succ_of_le H)
-}
-
-theorem or_imp_decompose {A B C D: Prop}: 
-  (A -> C) ∧ (B -> D) -> A ∨ B -> C ∨ D 
+theorem or_imp_decompose {A B C D: Prop}:
+  (A -> C) ∧ (B -> D) -> A ∨ B -> C ∨ D
   := by {
     intro ⟨F, G⟩;
     intro H;
@@ -351,27 +18,13 @@ theorem or_imp_decompose {A B C D: Prop}:
     | inr H => exact Or.inr (G H)
   }
 
-theorem and_imp_decompose {A B C: Prop}: (A ∧ B -> C) = (A -> B -> C) 
+theorem and_imp_decompose {A B C: Prop}: (A ∧ B -> C) = (A -> B -> C)
   := propext (Iff.intro (λF a b => F ⟨a, b⟩) (λF ⟨a, b⟩ => F a b))
 
-theorem Nat.gt_sub_succ: n ≤ m -> (Nat.succ m) - n = Nat.succ (m - n) := by {
-  revert n;
-  induction m with
-  | zero => intro n H; cases H; rfl
-  | succ m I =>
-    intro n;
-    cases n with
-    | zero => intro; simp
-    | succ n =>
-      intro H
-      simp only [Nat.succ_sub_succ_eq_sub]
-      exact I (Nat.le_of_succ_le_succ H)
-}
-
 theorem monorecursor
-  : 
+  :
   @Eq.rec A x F D y p =
-  @Eq.rec (Type) (F x rfl) (λA _ => A) D (F y p) p'  
+  @Eq.rec (Type) (F x rfl) (λA _ => A) D (F y p) p'
   := by {
     cases p;
     cases p';
@@ -379,27 +32,27 @@ theorem monorecursor
   }
 
 theorem rec_to_cast
-  : 
+  :
   @Eq.rec A x F D y p =
-  cast p' D 
+  cast p' D
   := by {
     cases p;
     rfl
   }
 
 theorem mp_to_cast
-  : 
+  :
   Eq.mp p D =
-  cast p D 
+  cast p D
   := by {
     cases p;
     rfl
   }
 
 theorem rec_to_cast'
-  : 
+  :
   @Eq.rec A x F D y p =
-  cast (by cases p; rfl) D 
+  cast (by cases p; rfl) D
   := by {
     cases p;
     rfl
@@ -420,7 +73,7 @@ theorem pair_mono_transport
   :
   @Eq.rec (Type) (Prod A B) (λA _ => A) (x, y) (Prod C D) Ppair =
   (
-    @Eq.rec (Type) A (λA _ => A) x C PA, 
+    @Eq.rec (Type) A (λA _ => A) x C PA,
     @Eq.rec (Type) B (λA _ => A) y D PB
   )
   := by {
@@ -466,7 +119,7 @@ theorem cast_none' (p: A = B) (q)
     cases p;
     rfl
   }
- 
+
 theorem cast_inl {A B C D: Type} {a: A} (p: A = C) (p': B = D)
   : cast (by rw [p, p']) (@Sum.inl A B a) = @Sum.inl C D (cast p a)
   := by {
@@ -474,7 +127,7 @@ theorem cast_inl {A B C D: Type} {a: A} (p: A = C) (p': B = D)
     cases p';
     rfl
   }
- 
+
 theorem cast_inr {A B C D: Type} {b: B} (p: A = C) (p': B = D)
   : cast (by rw [p, p']) (@Sum.inr A B b) = @Sum.inr C D (cast p' b)
   := by {
@@ -482,7 +135,7 @@ theorem cast_inr {A B C D: Type} {b: B} (p: A = C) (p': B = D)
     cases p';
     rfl
   }
-  
+
 theorem cast_inl' {A B C D: Type} {a: A} (p: A = C) (p': B = D) (p'')
   : cast p'' (@Sum.inl A B a) = @Sum.inl C D (cast p a)
   := by {
@@ -490,7 +143,7 @@ theorem cast_inl' {A B C D: Type} {a: A} (p: A = C) (p': B = D) (p'')
     cases p';
     rfl
   }
- 
+
 theorem cast_inr' {A B C D: Type} {b: B} (p: A = C) (p': B = D) (p'')
   : cast p'' (@Sum.inr A B b) = @Sum.inr C D (cast p' b)
   := by {
@@ -504,23 +157,23 @@ theorem cast_tri {B: A -> Type} {D: C -> Type}
   (x: C)
   (p: C = A)
   (p': p ▸ B = D)
-  : @cast 
-    (B (p ▸ x)) (D x) 
-    (by cases p; cases p'; rfl) 
-    (f (cast p x)) = 
+  : @cast
+    (B (p ▸ x)) (D x)
+    (by cases p; cases p'; rfl)
+    (f (cast p x)) =
     (@cast ((a: A) -> B a) ((c: C) -> D c) (by cases p; cases p'; rfl) f) x
   := by {
     cases p;
     cases p';
     rfl
   }
-  
+
 theorem cast_tri' {A B C D}
   (x: A)
   (f: C -> D)
   (p: A = C)
   (p': B = D)
-  : cast p'.symm (f (cast p x)) 
+  : cast p'.symm (f (cast p x))
   = (@cast (C -> D) (A -> B) (by cases p; cases p'; rfl) f) x
   := by {
     cases p;
@@ -533,7 +186,7 @@ theorem cast_tri'' {A B C D}
   (f: C -> D)
   (p: A = C)
   (p': B = D)
-  : cast p' ((@cast (C -> D) (A -> B) (by cases p; cases p'; rfl) f) x) 
+  : cast p' ((@cast (C -> D) (A -> B) (by cases p; cases p'; rfl) f) x)
   = f (cast p x)
   := by {
     cases p;
@@ -573,7 +226,7 @@ theorem equiv_prop_split {P Q R S: Prop}
   (q: Q = R) (p: P = Q) (r: R = S):
   P = S
   := by {
-    cases p; cases q; cases r; rfl 
+    cases p; cases q; cases r; rfl
   }
 
 theorem equiv_and_split {P Q R: Prop}:
@@ -597,8 +250,8 @@ theorem cast_not_none_is_not_none {p: Option A = Option B} (p': A = B):
   (cast p a ≠ none) = (a ≠ none)
   := by {
     cases a with
-    | some a => 
-      apply propext; 
+    | some a =>
+      apply propext;
       --TODO: report unused variable bug here
       apply Iff.intro <;> intro _
       . simp
@@ -613,7 +266,7 @@ theorem equiv_arrow_helper {A B C D: Prop}
   : A = C -> B = D -> (A -> B) = (C -> D)
   := by {
     intro H H';
-    cases H; cases H'; rfl 
+    cases H; cases H'; rfl
   }
 
 theorem equiv_arrow_helper' {A B C D: Prop}
@@ -626,7 +279,7 @@ theorem equiv_arrow_helper' {A B C D: Prop}
     {
       intro H'' a;
       rw [<-H' a]
-      exact H'' a 
+      exact H'' a
     }
     {
       intro H'' a;
@@ -635,14 +288,14 @@ theorem equiv_arrow_helper' {A B C D: Prop}
     }
   }
 
-theorem cast_app 
-  (A: Type) 
+theorem cast_app
+  (A: Type)
   (B: A -> Type)
   (B': A -> Type)
   (HB: B = B')
   (a: A)
   (f: (a: A) -> B a):
-  (@cast ((a: A) -> B a) ((a: A) -> B' a) (by rw [HB]) f) a 
+  (@cast ((a: A) -> B a) ((a: A) -> B' a) (by rw [HB]) f) a
   = cast (by rw [HB]) (f a)
   := by {
     cases HB; rfl
@@ -673,7 +326,7 @@ theorem cast_app_pull_in {A B C}
   (a: A)
   (H: (A -> B) = (A -> C))
   (H': B = C):
-  (@cast (A -> B) (A -> C) H f) a 
+  (@cast (A -> B) (A -> C) H f) a
   = cast H' (f a)
   := by {
     cases H';
@@ -688,7 +341,7 @@ theorem cast_app_pull_in_dep
   (H: ((a: A) -> B a) = ((a: A) -> C a))
   (H')
   (H'': B = C):
-  (@cast ((a: A) -> B a) ((a: A) -> C a) H f) a 
+  (@cast ((a: A) -> B a) ((a: A) -> C a) H f) a
   = cast H' (f a)
   := by {
     cases H'';
@@ -725,7 +378,7 @@ theorem cast_result
   (A B C: Type)
   (f: A -> B)
   (H: B = C):
-  (λx => cast (by rw [H]) (f x)) = cast (by rw [H]) f 
+  (λx => cast (by rw [H]) (f x)) = cast (by rw [H]) f
   := by {
     cases H;
     rfl
@@ -747,16 +400,16 @@ theorem existential_helper {A: Prop} {B C: A -> Prop}
       intro ⟨Ha, Hb⟩;
       cases H with
       | inl => contradiction
-      | inr H => rw [<-H]; exact ⟨Ha, Hb⟩ 
+      | inr H => rw [<-H]; exact ⟨Ha, Hb⟩
     }
     {
       intro ⟨Ha, Hc⟩;
       cases H with
       | inl => contradiction
-      | inr H => rw [H]; exact ⟨Ha, Hc⟩ 
+      | inr H => rw [H]; exact ⟨Ha, Hc⟩
     }
   }
-  
+
 theorem forall_helper {A: Type} {B C: A -> Prop}
   (H: ∀x: A, B x = C x): (∀x: A, B x) = (∀x: A, C x)
   := by {
@@ -811,12 +464,12 @@ theorem existential_forall_helper_dep {A B: Type} {C: A -> Prop} {D: B -> Prop}
   }
 
   theorem cast_app_prop
-  (A B: Sort u) 
+  (A B: Sort u)
   (f: A -> Prop)
   (b: B)
   (H: (A -> Prop) = (B -> Prop))
   (H': B = A):
-  (cast H f) b 
+  (cast H f) b
   = f (cast H' b)
   := by {
     cases H';
@@ -862,9 +515,9 @@ theorem cast_app_dep_one
   }
 
 theorem cast_app_dep_two
-  {A: Sort u0} 
+  {A: Sort u0}
   {B: A -> Sort u1}
-  {C: (a: A) -> B a -> Sort u2} 
+  {C: (a: A) -> B a -> Sort u2}
   {R: Sort v}
   (f: (a: A) -> (b: B a) -> C a b -> R)
   (a a': A)
@@ -881,10 +534,10 @@ theorem cast_app_dep_two
   }
 
 theorem cast_app_dep_three
-  {A: Sort u0} 
+  {A: Sort u0}
   {B: A -> Sort u1}
   {C: (a: A) -> B a -> Sort u2}
-  {D: (a: A) -> (b: B a) -> (c: C a b) -> Sort u3} 
+  {D: (a: A) -> (b: B a) -> (c: C a b) -> Sort u3}
   {R: Sort v}
   (f: (a: A) -> (b: B a) -> (c: C a b) -> D a b c -> R)
   (a a': A)
@@ -905,11 +558,11 @@ theorem cast_app_dep_three
   }
 
 theorem cast_app_dep_four
-  {A: Sort u0} 
+  {A: Sort u0}
   {B: A -> Sort u1}
   {C: (a: A) -> B a -> Sort u2}
   {D: (a: A) -> (b: B a) -> (c: C a b) -> Sort u3}
-  {E: (a: A) -> (b: B a) -> (c: C a b) -> (d: D a b c) -> Sort u4} 
+  {E: (a: A) -> (b: B a) -> (c: C a b) -> (d: D a b c) -> Sort u4}
   {R: Sort v}
   (f: (a: A) -> (b: B a) -> (c: C a b) -> (d: D a b c) -> E a b c d -> R)
   (a a': A)
